Pset3 lookup_insert done

pset03_ContainersAndHOFs/Pset3.v
@@ -66,17 +66,35 @@ Module Impl.
   Lemma compose_id_l : forall A B (f: A -> B),
       id ∘ f = f.
   Proof.
-  Admitted.
+      intros.
+      apply fun_ext.
+      unfold compose.
+      intros x.
+      unfold id.
+      equality.
+  Qed.
 
   Lemma compose_id_r : forall A B (f: A -> B),
       f ∘ id = f.
   Proof.
-  Admitted.
+      intros.
+      apply fun_ext.
+      unfold compose.
+      intro x.
+      unfold id.
+      equality.
+   Qed.
+
 
   Lemma compose_assoc : forall A B C D (f: A -> B) (g: B -> C) (h: C -> D),
       h ∘ (g ∘ f) = h ∘ g ∘ f.
   Proof.
-  Admitted.
+      intros.
+      apply fun_ext.
+      unfold compose.
+      intros x.
+      equality.
+   Qed.
 
   (* The selfCompose function takes a function and applies this function n times
      to the argument. There are different ways of defining it, but let's
@@ -96,14 +114,15 @@ Module Impl.
      saying "to raise [base] to the power [e], apply the function that multiplies
      its argument by [base] to [1] [e] times".
      Define [exp] using [selfCompose] and [Nat.mul]. *)
-  Definition exp(base e: nat): nat. Admitted.
+  Definition exp(base e: nat): nat := 
+      selfCompose (Nat.mul base) e 1.
 
   (* Once you define [exp], you can replace [Admitted.] below by [Proof. equality. Qed.] *)
-  Lemma test_exp_2_3: exp 2 3 = 8. Admitted.
-  Lemma test_exp_3_2: exp 3 2 = 9. Admitted.
-  Lemma test_exp_4_1: exp 4 1 = 4. Admitted.
-  Lemma test_exp_5_0: exp 5 0 = 1. Admitted.
-  Lemma test_exp_1_3: exp 1 3 = 1. Admitted.
+  Lemma test_exp_2_3: exp 2 3 = 8. Proof. equality. Qed.
+  Lemma test_exp_3_2: exp 3 2 = 9. Proof. equality. Qed.
+  Lemma test_exp_4_1: exp 4 1 = 4. Proof. equality. Qed.
+  Lemma test_exp_5_0: exp 5 0 = 1. Proof. equality. Qed.
+  Lemma test_exp_1_3: exp 1 3 = 1. Proof. equality. Qed.
 
   (* And here's another example to illustrate [selfCompose]. Make sure you understand
      why its result is 256. *)
@@ -119,7 +138,15 @@ Module Impl.
      is the left inverse of the function that adds two to its argument. *)
   Example plus2minus2: left_inverse (fun (x: nat) => x + 2) (fun (x: nat) => x - 2).
   Proof.
-  Admitted.
+    unfold left_inverse.
+    unfold compose.
+    Search (_ + ?x - ?x).
+    unfold id.
+    apply fun_ext.
+    intros x.
+    rewrite Nat.add_sub.
+    equality.
+  Qed.
 
   (* On the other hand, note that the other direction does not hold, because
      if a subtraction on natural numbers underflows, it just returns 0, so
@@ -127,7 +154,20 @@ Module Impl.
      so it can't have a left inverse. *)
   Example minus2plus2: ~ left_inverse (fun (x: nat) => x - 2) (fun (x: nat) => x + 2).
   Proof.
-  Admitted.
+    unfold left_inverse.
+    intros H.
+    assert (H0: ((fun x => x+2) ∘ (fun x => x- 2)) 0 = id 0).
+    {
+     rewrite H. equality.
+    }
+    unfold compose in H0.
+    unfold id in H0.
+    Search (0 - _).
+    rewrite Nat.sub_0_l in H0.
+    simpl in H0.
+    discriminate H0.
+  Qed.
+
 
   (* Let us make the intuition from the previous paragraph more
      concrete, by proving that a function that is not injective
@@ -140,7 +180,23 @@ Module Impl.
       left_inverse f g ->
       (forall x y, f x = f y -> x = y).
   Proof.
-  Admitted.
+    intros f g H x y Hfxfy.
+    unfold left_inverse in H.
+    assert (H1: g (f x) = g (f y)).
+    {
+      rewrite Hfxfy. equality.
+    }
+
+   assert (H2: (g ∘ f) x = (g ∘ f) y).
+   {
+     unfold compose. 
+     assumption.
+   }
+
+   rewrite H in H2.
+   unfold id in H2.
+   assumption.
+  Qed.
 
   (* Bonus question (no points): can you prove the reverse;
      i.e., can you prove that all injective functions have left
@@ -151,7 +207,12 @@ Module Impl.
      type arguments explicitly, because otherwise Coq would not be able to infer them." *)
   Lemma left_inverse_id: forall A, left_inverse (@id A) (@id A).
   Proof.
-  Admitted.
+    intros.
+    unfold left_inverse.
+    unfold compose.
+    unfold id.
+    equality.
+  Qed.
 
 
   (* Now we can start proving interesting facts about inverse functions: *)
@@ -161,7 +222,33 @@ Module Impl.
       left_inverse f g ->
       left_inverse (selfCompose f n) (selfCompose g n).
   Proof.
-  Admitted.
+    unfold left_inverse.
+    induct n.
+    - simplify. apply left_inverse_id.
+    - simplify.
+ 
+    assert (Hg: forall n': nat, g ∘ selfCompose g n' = selfCompose g n' ∘ g).
+    {
+      induct n'.
+      - simplify.
+        rewrite compose_id_l.
+        rewrite compose_id_r.
+        equality.
+      - simplify.
+        rewrite IHn' at 1.
+        auto.
+    }
+
+    rewrite Hg.
+    Search ( _∘ _ ∘ _).
+    rewrite compose_assoc. 
+    rewrite <- compose_assoc with (h := selfCompose g n).
+    rewrite H.
+    rewrite compose_id_r.
+    apply IHn.
+    assumption.
+  Qed.
+  
 
   (** ** Polymorphic container types *)
 
@@ -193,8 +280,7 @@ Module Impl.
   Definition bitwise_trie A := tree (option A).
 
   (* Define [lookup] such that [lookup k t] looks up the
-    Fixpoint lookup {A} (k : list bool) (t : bitwise_trie A) {struct t} : option A :=
-    Admitted. * map entry corresponding to the key [k : list bool] in the
+   * map entry corresponding to the key [k : list bool] in the
    * bitwise trie [t : bitwise_trie A].
    *
    * Look at the examples below to get a better sense of what
@@ -207,10 +293,9 @@ Module Impl.
     | Leaf, _ => None
     | Node l None r, [] => None
     | Node l (Some v) r, [] => Some v
-    | Node l _ r, true::ks =>  lookup ks l
-    | Node l _ r, false::ks => lookup ks r
+    | Node l _ r, true::k' =>  lookup k' l
+    | Node l _ r, false::k' => lookup k' r
     end.
-
 
   Example lookup_example1 : lookup [] (Node Leaf (None : option nat) Leaf) = None.
   Proof.
@@ -230,11 +315,11 @@ Module Impl.
   Theorem lookup_empty {A} (k : list bool)
     : lookup k (Leaf : bitwise_trie A) = None.
   Proof.
-    simplify. 
+    simplify.
     case k.
     - equality.
-    - equality. 
-  Qed.
+    - equality.
+  Qed.   
 
   (* HINT 3 (see Pset3Sig.v) *)
 
@@ -254,21 +339,69 @@ Module Impl.
    * that creates a singleton tree (a tree containing a single
    * key-value pair).
    *)
+  Fixpoint build_singleton {A} (k : list bool) (v : option A) : bitwise_trie A :=
+     match k with
+     | [] => Node Leaf v Leaf
+     | x :: k' => let branch := build_singleton k' v in
+                  if x then Node branch None Leaf
+                  else Node Leaf None branch
+     end.
+
   Fixpoint insert {A} (k : list bool) (v : option A) (t : bitwise_trie A) {struct t}
-    : bitwise_trie A. Admitted.
+    : bitwise_trie A :=
+    match t with
+    | Leaf => build_singleton k v
+    | Node l old_v r =>
+      match k with
+      | [] => Node l v r
+      | x :: k' => if x then Node (insert k' v l) old_v r
+                   else Node l old_v (insert k' v r)
+      end
+    end.
 
   Example insert_example1 : lookup [] (insert [] None (Node Leaf (Some 0) Leaf)) = None.
   Proof.
-  Admitted.
+    simplify. equality.
+  Qed.
 
   Example insert_example2 : lookup [] (insert [true] (Some 2) (Node Leaf (Some 0) Leaf)) = Some 0.
   Proof.
-  Admitted.
+    simplify. equality.
+  Qed.
 
   Theorem lookup_insert {A} (k : list bool) (v : option A) (t : bitwise_trie A) :
     lookup k (insert k v t) = v.
   Proof.
-  Admitted.
+    generalize dependent v.
+    generalize dependent k.
+    induct t.
+    - (* Case: t is Leaf *)
+      simplify. induct k.
+      + (* Case: k is [] *)
+        simplify. 
+        case v; equality.
+      + (* Case: k is x::k' *)  
+        simplify. case a; simplify.
+        * apply IHk.
+        * apply IHk.
+    - (* Case: t is Node *)
+      simplify. case k. 
+      + (* Case: k is [] *)
+        simplify.
+        case v; equality.
+      + (* Case: k is x::k' *)
+        intros. case b.
+        * simplify.
+          case d; simplify.
+            apply IHt1.
+            apply IHt1.
+        * simplify.
+          case d; simplify.
+            apply IHt2.
+            apply IHt2.
+  Qed.
+
+
 
   (* Define an operation to "merge" that takes two bitwise tries and merges
    * them together. The [merge] definition should combine two bitwise tries, 
